theories/typing/uninit.v
@@ -6,15 +6,23 @@ Set Default Proof Using "Type".
 Section uninit.
   Context `{!typeG Σ}.
 
-  Program Definition uninit1: type unit :=
+  Program Definition uninit1: type () :=
     {| pt_size := 1;  pt_own _ _ vl := ⌜∃v, vl = [v]⌝; |}%I.
-  Next Obligation. by iIntros "* [%->]". Qed.
+  Next Obligation. by iIntros "*[%->]". Qed.
+
+  Definition uninit (n: nat) : type () := <{unique}> [uninit1; n].
+
+End uninit.
+
+Notation "↯" := (uninit) : lrust_type_scope.
+
+Section typing.
+  Context `{!typeG Σ}.
 
   Global Instance uninit1_send: Send uninit1. Proof. done. Qed.
+  Global Instance uninit1_sync: Sync uninit1. Proof. done. Qed.
 
-  Definition uninit n : type unit := <{unique}> (array n uninit1).
-
-  Lemma uninit_own n vπ d tid vl : (uninit n).(ty_own) vπ d tid vl ⊣⊢ ⌜length vl = n⌝.
+  Lemma uninit_own n vπ d tid vl : (↯ n).(ty_own) vπ d tid vl ⊣⊢ ⌜length vl = n⌝.
   Proof.
     rewrite mod_ty_own. move: vl. elim: n=> [|n IH] vl.
     - by rewrite mod_ty_own length_zero_iff_nil.
@@ -24,14 +32,14 @@ Section uninit.
         iPureIntro. split; [done|]. split; [|done]. exists (). split; by [|exists v].
   Qed.
 
-  Lemma uninit_0_unit: uninit 0 ≡ unit_ty.
+  Lemma uninit_0_unit: (↯ 0 ≡ ())%T.
   Proof.
     split=>// *; [rewrite !mod_ty_own|rewrite !mod_ty_shr];
     by rewrite compose_assoc semi_iso.
   Qed.
 
   Lemma uninit_plus_prod E L m n :
-    eqtype E L unique unique (uninit (m + n)) (uninit m * uninit n).
+    eqtype E L unique unique (↯ (m + n)) (↯ m * ↯ n).
   Proof.
     have [->->]:
       @unique (() → ()*()) _ = prod_map unique unique ∘ (@pvsep () m n) ∘ unique ∧
@@ -41,4 +49,4 @@ Section uninit.
     { apply array_plus_prod. } apply prod_eqtype; apply mod_ty_inout, _.
   Qed.
 
-End uninit.
+End typing.
