theories/typing/maybe_uninit.v
@@ -1,0 +1,119 @@
+Require Import FunctionalExtensionality Equality.
+From lrust.typing Require Export type.
+
+Section maybe_uninit.
+  Context `{!typeG Σ}.
+
+  Local Lemma maybe_uninit_mt {A} (ty: _ A) vπ d tid l q :
+    (l ↦∗{q}: λ vl, ⌜vπ = const None ∧ length vl = ty.(ty_size)⌝ ∨
+      ∃vπ', ⌜vπ = Some ∘ vπ'⌝ ∗ ty.(ty_own) vπ' d tid vl)%I ⊣⊢
+    ⌜vπ = const None⌝ ∗ l ↦∗{q}: (λ vl, ⌜length vl = ty.(ty_size)⌝) ∨
+    ∃vπ', ⌜vπ = Some ∘ vπ'⌝ ∗ l ↦∗{q}: ty.(ty_own) vπ' d tid.
+  Proof. iSplit.
+    - iIntros "(%vl&?&[[%%]|(%vπ'&%&?)])". { iLeft. iSplit; [done|]. iExists vl.
+      by iFrame. } iRight. iExists vπ'. iSplit; [done|]. iExists vl. iFrame.
+    - iIntros "[(%&%vl&Mt&%)|(%vπ'&%&%vl&Mt&?)]". { iExists vl. iFrame "Mt". by iLeft. }
+      iExists vl. iFrame "Mt". iRight. iExists vπ'. by iSplit.
+  Qed.
+
+  Program Definition maybe_uninit {A} (ty: type A) : type (option A) := {|
+    ty_size := ty.(ty_size);  ty_lfts := ty.(ty_lfts);  ty_E := ty.(ty_E);
+    ty_own vπ d tid vl :=
+      ⌜vπ = const None ∧ length vl = ty.(ty_size)⌝ ∨
+      ∃vπ', ⌜vπ = Some ∘ vπ'⌝ ∗ ty.(ty_own) vπ' d tid vl;
+    ty_shr vπ d κ tid l :=
+      ⌜vπ = const None⌝ ∨ ∃vπ', ⌜vπ = Some ∘ vπ'⌝ ∗ ty.(ty_shr) vπ' d κ tid l;
+  |}%I.
+  Next Obligation. iIntros "* [[_$]|(%&_&?)]". by rewrite ty_size_eq. Qed.
+  Next Obligation.
+    move=> *. iIntros "[?|(%vπ&?&?)]"; [by iLeft|iRight]. iExists vπ.
+    iSplit; [done|]. by iApply ty_own_depth_mono.
+  Qed.
+  Next Obligation.
+    move=> *. iIntros "[?|(%vπ&?&?)]"; [by iLeft|iRight]. iExists vπ.
+    iSplit; [done|]. by iApply ty_shr_depth_mono.
+  Qed.
+  Next Obligation.
+    move=> *. iIntros "#? [?|(%vπ&?&?)]"; [by iLeft|iRight]. iExists vπ.
+    iSplit; [done|]. by iApply ty_shr_lft_mono.
+  Qed.
+  Next Obligation.
+    move=> *. iIntros "#LFT In Bor Tok". rewrite maybe_uninit_mt.
+    iMod (bor_or with "LFT Bor") as "[Bor|Bor]"; first done.
+    { iApply step_fupdN_full_intro.
+      iMod (bor_sep_persistent with "LFT Bor Tok") as "(>->&?&$)"; by [|iLeft]. }
+    iMod (bor_exists_tok with "LFT Bor Tok") as (vπ) "[Bor Tok]"; [done|].
+    iMod (bor_sep_persistent with "LFT Bor Tok") as "(>->& Bor & Tok)"; [done|].
+    iMod (ty_share with "LFT In Bor Tok") as "Upd"; [done|].
+    iApply (step_fupdN_wand with "Upd"). iIntros "!> >[?$] !>". iRight.
+    iExists vπ. by iFrame.
+  Qed.
+  Next Obligation.
+    move=> *. iIntros "LFT In [[->%]|(%vπ &->& Own)] Tok".
+    { iApply step_fupdN_full_intro. iIntros "!>!>". iExists [], 1%Qp.
+      do 2 (iSplit; [done|]). iIntros "_!>". iFrame "Tok". by iLeft. }
+    iMod (ty_own_proph with "LFT In Own Tok") as "Upd"; [done|].
+    iApply (step_fupdN_wand with "Upd"). iIntros "!> >(%ξs & %q &%& PTok & Close) !>".
+    iExists ξs, q. iSplit; [iPureIntro; by apply proph_dep_constr|].
+    iFrame "PTok". iIntros "PTok". iMod ("Close" with "PTok") as "[?$]".
+    iRight. iExists vπ. by iFrame.
+  Qed.
+  Next Obligation.
+    move=> *. iIntros "LFT In In' [->|(%vπ &->& Shr)] Tok".
+    { iApply step_fupdN_full_intro. iIntros "!>!>!>!>". iExists [], 1%Qp.
+      do 2 (iSplit; [done|]). iIntros "_!>". iFrame "Tok". by iLeft. }
+    iMod (ty_shr_proph with "LFT In In' Shr Tok") as "Upd"; [done|].
+    iIntros "!>!>". iApply (step_fupdN_wand with "Upd").
+    iIntros ">(%ξs & %q &%& PTok & Close) !>". iExists ξs, q.
+    iSplit; [iPureIntro; by apply proph_dep_constr|]. iFrame "PTok". iIntros "PTok".
+    iMod ("Close" with "PTok") as "[?$]". iRight. iExists vπ. by iFrame.
+  Qed.
+
+  Global Instance maybe_uninit_ne {A} : NonExpansive (@maybe_uninit A).
+  Proof. solve_ne_type. Qed.
+
+End maybe_uninit.
+
+Notation "?" := maybe_uninit : lrust_type_scope.
+
+Section typing.
+  Context `{!typeG Σ}.
+
+  Global Instance maybe_uninit_send {A} (ty: _ A) : Send ty → Send (? ty).
+  Proof. move=> Eq >/=. by setoid_rewrite Eq at 1. Qed.
+  Global Instance maybe_uninit_sync {A} (ty: _ A) : Sync ty → Sync (? ty).
+  Proof. move=> Eq >/=. by setoid_rewrite Eq at 1. Qed.
+
+  Lemma maybe_uninit_subtype {A B} (f: A → B) ty ty' E L :
+    subtype E L f ty ty' → subtype E L (option_map f) (? ty) (? ty').
+  Proof.
+    move=> Sub ?. iIntros "L". iDestruct (Sub with "L") as "#Sub".
+    iIntros "!> E". iDestruct ("Sub" with "E") as "(%&?& #InOwn & #InShr)".
+    do 2 (iSplit; [done|]). iSplit; iIntros "!> * /=".
+    - iIntros "[[->->]|(%vπ' &->&?)]"; [by iLeft|]. iRight. iExists (f ∘ vπ').
+      iSplit; [done|]. by iApply "InOwn".
+    - iIntros "[->|(%vπ' &->&?)]"; [by iLeft|]. iRight. iExists (f ∘ vπ').
+      iSplit; [done|]. by iApply "InShr".
+  Qed.
+  Lemma maybe_uninit_eqtype {A B} (f: A → B) g ty ty' E L :
+    eqtype E L f g ty ty' → eqtype E L (option_map f) (option_map g) (? ty) (? ty').
+  Proof. move=> [??]. split; by apply maybe_uninit_subtype. Qed.
+
+  Lemma into_maybe_uninit {A} (ty: _ A) E L : subtype E L Some ty (? ty).
+  Proof.
+    iIntros (?) "_!>_". iSplit; [done|]. iSplit; [by iApply lft_incl_refl|].
+    iSplit; iIntros "!> * ? /="; iRight; iExists vπ; by iFrame.
+  Qed.
+
+  Lemma maybe_uninit_join {A} (ty: _ A) E L :
+    subtype E L (option_join _) (? (? ty)) (? ty).
+  Proof.
+    iIntros (?) "_!>_". iSplit; [done|]. iSplit; [by iApply lft_incl_refl|].
+    iSplit; iIntros "!> * /=".
+    - iIntros "[[->->]|(%&->&[[->->]|(%vπ''&->&?)])]"; [by iLeft|by iLeft|].
+      iRight. iExists vπ''. by iFrame.
+    - iIntros "[->|(%&->&[->|(%vπ''&->&?)])]"; [by iLeft|by iLeft|].
+      iRight. iExists vπ''. by iFrame.
+  Qed.
+
+End typing.
